cat/io_specs_rollback.v
@@ -1,0 +1,72 @@
+Require Import VST.veric.juicy_extspec.
+Require Import VST.floyd.proofauto.
+Require Export VST.floyd.io_events.
+Require Export ITree.ITree.
+Require Export ITree.Eq.SimUpToTaus.
+Require Export ITree.Events.Nondeterminism.
+(* Import ITreeNotations. *) (* one piece conflicts with subp notation *)
+Notation "t1 >>= k2" := (ITree.bind t1 k2)
+  (at level 50, left associativity) : itree_scope.
+Notation "x <- t1 ;; t2" := (ITree.bind t1 (fun x => t2))
+  (at level 100, t1 at next level, right associativity) : itree_scope.
+Notation "t1 ;; t2" := (ITree.bind t1 (fun _ => t2))
+  (at level 100, right associativity) : itree_scope.
+Notation "' p <- t1 ;; t2" :=
+  (ITree.bind t1 (fun x_ => match x_ with p => t2 end))
+(at level 100, t1 at next level, p pattern, right associativity) : itree_scope.
+
+Definition stdin := 0%nat.
+Definition stdout := 1%nat.
+
+Instance Reflexive_sutt {E R} : RelationClasses.Reflexive (@sutt E R R eq).
+Proof. intro; apply eutt_sutt; reflexivity. Qed.
+
+Lemma or_case1 : forall {E R} `{nondetE -< E} a b, sutt eq a (or(R := R) a b).
+Proof.
+  intros; unfold or.
+Admitted.
+
+Lemma or_case2 : forall {E R} `{nondetE -< E} a b, sutt eq b (or(R := R) a b).
+Proof.
+  intros; unfold or.
+Admitted.
+Section specs.
+
+Context {E : Type -> Type} `{IO_event(file_id := nat) -< E}.
+
+(* If putchar fails, we shouldn't be forced to commit to writing. *)
+Definition putchar_spec :=
+  WITH c : byte, k : IO_itree, t : IO_itree
+  PRE [ 1%positive OF tint ]
+    PROP (sutt eq (write stdout c;; k) t)
+    LOCAL (temp 1%positive (Vubyte c))
+    SEP (ITREE t)
+  POST [ tint ]
+   EX i : int,
+    PROP (Int.signed i = -1 \/ Int.signed i = Byte.unsigned c)
+    LOCAL (temp ret_temp (Vint i))
+    SEP (ITREE (if eq_dec (Int.signed i) (-1) then t else k)).
+
+Definition getchar_spec :=
+  WITH k : byte -> IO_itree, t : IO_itree
+  PRE [ ]
+    PROP (sutt eq (r <- read stdin ;; k r) t)
+    LOCAL ()
+    SEP (ITREE t)
+  POST [ tint ]
+   EX i : int,
+    PROP (-1 <= Int.signed i <= Byte.max_unsigned)
+    LOCAL (temp ret_temp (Vint i))
+    SEP (ITREE (if eq_dec (Int.signed i) (-1) then t else k (Byte.repr (Int.signed i)))).
+
+(* Build the external specification. *)
+Definition IO_void_Espec : OracleKind := ok_void_spec (@IO_itree E).
+
+Definition IO_specs (ext_link : string -> ident) :=
+  [(ext_link "putchar"%string, putchar_spec); (ext_link "getchar"%string, getchar_spec)].
+
+Definition IO_Espec (ext_link : string -> ident) : OracleKind := add_funspecs IO_void_Espec ext_link (IO_specs ext_link).
+
+End specs.
+
+Ltac forward_call_io w := lazymatch goal with |- context[ITREE ?t] => forward_call (w, t); try reflexivity end.
